feat: still iterating on the definitions

Lean4Lean/Theory/EnvTyping.lean
@@ -7,44 +7,36 @@ namespace Lean4Lean
 
 open Lean (Name FVarId)
 
-def VDefVal.WF (env : VPreEnv) (ci : VDefVal) : Prop := env.HasType ci.uvars [] ci.value ci.type
+def VDefVal.WF (env : VEnv) (ci : VDefVal) : Prop := env.HasType ci.uvars [] ci.value ci.type
 
-inductive VDecl.WF : VPreEnv → VDecl → VEnv → Prop where
+inductive VDecl.WF : VEnv → VDecl → VEnv → Prop where
   | block :
-    env.env.addConst n none = some env' →
+    env.addConst n none = some env' →
     VDecl.WF env (.block n) env'
   | axiom :
-    ci.WF env.T →
-    env.env.addConst ci.name (some ci.toVConstant) = some env' →
+    ci.WF env.HasType →
+    env.addConst ci.name (some ci.toVConstant) = some env' →
     VDecl.WF env (.axiom ci) env'
   | def :
     ci.WF env →
-    env.env.addConst ci.name (some ci.toVConstant) = some env' →
+    env.addConst ci.name (some ci.toVConstant) = some env' →
     VDecl.WF env (.def ci) (env'.addDefEq ci.toDefEq)
   | opaque :
     ci.WF env →
-    env.env.addConst ci.name (some ci.toVConstant) = some env' →
+    env.addConst ci.name (some ci.toVConstant) = some env' →
     VDecl.WF env (.opaque ci) env'
   | example :
-    ci.WF env.T →
-    VDecl.WF env (.example ci) env.env
+    ci.WF env.HasType →
+    VDecl.WF env (.example ci) env
   | quot :
-    env.env.QuotReady →
-    env.env.addQuot = some env' →
+    env.QuotReady →
+    env.addQuot = some env' →
     VDecl.WF env .quot env'
   | induct :
-    decl.WF env.env →
-    env.env.addInduct decl = some env' →
+    decl.WF env →
+    env.addInduct decl = some env' →
     VDecl.WF env (.induct decl) env'
 
-def Typing.withEnv (env : VEnv) (T : Typing) : Typing :=
-  (VPreEnv.mk env T).HasType
-
-def Typing.empty : Typing := Typing.withEnv .empty fun _ _ _ _ => False
-
-inductive VEnv.WF : VEnv → List VDecl → Typing → Prop where
-  | empty : VEnv.WF .empty [] Typing.empty
-  | decl {env} :
-    VDecl.WF ⟨env, T⟩ d env' →
-    env.WF ds T →
-    env.WF (d::ds) (T.withEnv env')
+inductive VEnv.WF : VEnv → List VDecl → Prop where
+  | empty : VEnv.WF .empty []
+  | decl {env} : VDecl.WF env d env' → env.WF ds → env.WF (d::ds)
